Refactor

FinitePerm/Function/Basic.lean
@@ -6,75 +6,379 @@ Authors: Wrenna Robson
 module
 import Batteries.Tactic.Alias
 
-@[expose] public section
+public section
+
+variable {α : Sort u} {β : Sort v} {γ : Sort w}
 
 namespace Function
 
-/-- A function is called bijective if it is both injective and surjective. -/
-def Bijective (f : α → β) :=
-  Injective f ∧ Surjective f
+section Injective
 
-protected theorem Bijective.injective : Bijective f → Injective f := And.left
-protected theorem Bijective.surjective : Bijective f → Surjective f := And.right
+variable {f : α → β} {g g' : γ → α}
 
-theorem bijective_of_injective_of_surjective : Injective f → Surjective f → Bijective f :=
-  And.intro
+@[grind =>]
+theorem Injective.eq_of_comp_left_eq (hf : f.Injective) : f ∘ g = f ∘ g' → g = g' := by
+  simp only [funext_iff, comp_apply, hf.eq_iff, imp_self]
+
+@[simp] theorem Injective.comp_left_cancel (hf : f.Injective) :
+    f ∘ g = f ∘ g' ↔ g = g' := ⟨hf.eq_of_comp_left_eq, Eq.rec rfl⟩
+
+end Injective
+
+section Surjective
+
+variable {f : α → β} {g g' : β → γ}
+
+protected theorem Surjective.forall (hf : Surjective f) {p : β → Prop} :
+    (∀ y, p y) ↔ ∀ x, p (f x) :=
+  ⟨fun h x => h (f x), fun h y => let ⟨x, hx⟩ := hf y; hx ▸ h x⟩
+
+protected theorem Surjective.exists (hf : Surjective f) {p : β → Prop} :
+    (∃ y, p y) ↔ ∃ x, p (f x) :=
+  ⟨fun ⟨y, hy⟩ => let ⟨x, hx⟩ := hf y; ⟨x, hx ▸ hy⟩, fun ⟨x, hx⟩ => ⟨f x, hx⟩⟩
+
+@[grind =>]
+theorem Surjective.eq_of_comp_right_eq (hf : f.Surjective) : g ∘ f = g' ∘ f → g = g' := by
+  simp only [funext_iff, comp_apply, hf.forall, imp_self]
+
+@[simp] theorem Surjective.comp_right_cancel (hf : f.Surjective) :
+    g ∘ f = g' ∘ f ↔ g = g' := ⟨hf.eq_of_comp_right_eq, Eq.rec rfl⟩
+
+theorem Surjective.nonempty_fun (h : f.Surjective) : Nonempty (β → α) :=
+  ⟨(Exists.choose <| h ·)⟩
+
+theorem Surjective.nonempty (h : f.Surjective) [Nonempty β] :
+    Nonempty α := ⟨Exists.choose (h Classical.ofNonempty)⟩
+
+end Surjective
+
+/-- A function is *bijective* just when it is both injective and surjective. -/
+structure Bijective (f : α → β) where private mk ::
+  protected injective : Injective f
+  protected surjective : Surjective f
+
+/-- A pair of functions `(f, g)` form an equivalence when they are mutual two-sided inverses,
+i.e. `f ∘ g = id` and `g ∘ f = id`. -/
+structure Inverse (f : α → β) (g : β → α) where private mk ::
+  protected leftInverse : f.LeftInverse g
+  protected rightInverse : f.RightInverse g
+
+@[expose] def HasInverse {α β} (f : α → β) : Prop := Exists fun finv : β → α => Inverse finv f
+
+@[expose, grind, implicit_reducible] def Idempotent (f : α → α) : Prop := ∀ i, f (f i) = f i
+
+def inclusion (f : α → β) : Subtype (∃ a, f a = ·) → β := Subtype.val
+@[expose, grind] def restrict (f : α → β) : α → Subtype (∃ a, f a = ·) := fun i => ⟨f i, ⟨i, rfl⟩⟩
+
+section Restrict
+
+variable {f : α → β}
+
+@[simp] theorem val_restrict : (f.restrict i).val = f i := rfl
+
+@[simp, grind =] theorem val_comp_restrict : Subtype.val ∘ f.restrict = f := rfl
+
+end Restrict
+
+section Bijective
+
+attribute [grind =>] Bijective.injective Bijective.surjective
+
+variable {f : α → β}
+
+@[grind =>]
+theorem bijective_of_injective_of_surjective (hi : f.Injective) (hs : f.Surjective) :
+  f.Bijective := ⟨hi, hs⟩
 
 protected alias Injective.bijective_of_surjective := bijective_of_injective_of_surjective
 
 protected alias Surjective.bijective_of_injective := bijective_of_injective_of_surjective
 
-/-- A pair of functions `(f, g)` is a *splitting* (implicitly, of the identity) when `f` is a left
-inverse to`g`, i.e. `f ∘ g = id`. -/
-def IsSplitting (f : α → β) (g : β → α) := ∀ i, f (g i) = i
+theorem bijective_iff_injective_surjective : Bijective f ↔ f.Injective ∧ f.Surjective :=
+  ⟨fun h => And.intro h.injective h.surjective, fun ⟨hi, hs⟩ => hi.bijective_of_surjective hs⟩
 
-theorem IsSplitting.comp_eq_id (h : IsSplitting f g) : f ∘ g = id := funext h
+@[simp] theorem Bijective.comp_left_cancel (hf : f.Bijective) :
+    f ∘ g = f ∘ g' ↔ g = g' := hf.injective.comp_left_cancel
 
-theorem IsSplitting.injective : IsSplitting f g → Injective g := fun h i j hij =>
-  (h i).symm.trans <| (congrArg f hij).trans (h j)
+@[simp] theorem Bijective.comp_right_cancel (hf : f.Bijective) :
+    g ∘ f = g' ∘ f ↔ g = g' := hf.surjective.comp_right_cancel
 
-theorem IsSplitting.surjective : IsSplitting f g → Surjective f := fun h i => ⟨g i, h i⟩
+@[grind =>]
+theorem Bijective.eq_of_comp_left_eq (hf : f.Bijective) : f ∘ g = f ∘ g' → g = g' :=
+  hf.injective.eq_of_comp_left_eq
 
-theorem isSplitting_of_isSplitting_of_injective :
-    IsSplitting f g → Injective f → IsSplitting g f := fun h => (· <| h <| f <| ·)
+@[grind =>]
+theorem Bijective.eq_of_comp_right_eq (hf : f.Bijective) : g ∘ f = g' ∘ f → g = g' :=
+  hf.surjective.eq_of_comp_right_eq
 
-theorem isSplitting_of_isSplitting_of_surjective :
-    IsSplitting f g → Surjective g → IsSplitting g f :=
-  fun h => (let ⟨y, hy⟩ := · ·; hy ▸ congrArg g (h y))
+end Bijective
 
-alias IsSplitting.isSplitting_of_surjective := isSplitting_of_isSplitting_of_surjective
-alias IsSplitting.isSplitting_of_injective := isSplitting_of_isSplitting_of_injective
-alias Injective.isSplitting_of_isSplitting := isSplitting_of_isSplitting_of_injective
-alias Surjective.isSplitting_of_isSplitting := isSplitting_of_isSplitting_of_surjective
+section LeftInverse
 
-/-- A pair of functions `(f, g)` form an equivalence when they are mutual two-sided inverses,
-i.e. `f ∘ g = id` and `g ∘ f = id`. -/
-def IsEquiv (f : α → β) (g : β → α) := IsSplitting f g ∧ IsSplitting g f
+variable {α : Sort u} {β : Sort v} {f : α → β} {g g' : β → α}
 
-theorem IsEquiv.symm : IsEquiv f g → IsEquiv g f := And.symm
-theorem isEquiv_comm : IsEquiv f g ↔ IsEquiv g f := And.comm
+theorem LeftInverse.apply_apply (h : f.LeftInverse g) (i : β) : f (g i) = i := h i
 
-protected theorem IsEquiv.isSplitting_left : IsEquiv f g → IsSplitting f g := And.left
-protected theorem IsEquiv.isSplitting_right : IsEquiv f g → IsSplitting g f := And.right
+theorem leftInverse_def : f.LeftInverse g ↔ ∀ i, f (g i) = i := Iff.rfl
 
-theorem isEquiv_of_isSplitting_of_isSplitting :
-    IsSplitting f g → IsSplitting g f → IsEquiv f g := And.intro
+@[grind =>] theorem LeftInverse.comp_eq_id (h : f.LeftInverse g) : f ∘ g = id := funext h
 
-protected alias IsSplitting.isEquiv_of_isSplitting := isEquiv_of_isSplitting_of_isSplitting
+@[grind =>]
+theorem LeftInverse.comp_rev_idempotent (h : f.LeftInverse g) : (g ∘ f).Idempotent :=
+  (congrArg g <| h.apply_apply <| f ·)
 
-theorem isEquiv_of_isSplitting_of_surjective : IsSplitting f g → Surjective g ->
-    IsEquiv f g := fun hfg => hfg.isEquiv_of_isSplitting ∘ hfg.isSplitting_of_surjective
+theorem leftInverse_iff_comp_eq_id : f.LeftInverse g ↔ f ∘ g = id :=
+  ⟨LeftInverse.comp_eq_id, fun h => congrFun h⟩
 
-theorem isEquiv_of_isSplitting_of_injective : IsSplitting f g → Injective f ->
-    IsEquiv f g := fun hfg => hfg.isEquiv_of_isSplitting ∘ hfg.isSplitting_of_injective
+attribute [grind =>] LeftInverse.injective
 
-alias IsSplitting.isEquiv_of_surjective := isEquiv_of_isSplitting_of_surjective
-alias Surjective.isEquiv_of_isSplitting := isEquiv_of_isSplitting_of_surjective
-alias IsSplitting.isEquiv_of_injective := isEquiv_of_isSplitting_of_injective
-alias Injective.isEquiv_of_isSplitting := isEquiv_of_isSplitting_of_injective
+@[grind =>] theorem LeftInverse.surjective : f.LeftInverse g → Surjective f := fun h i => ⟨g i, h i⟩
 
-theorem IsEquiv.bijective_right : IsEquiv f g → Bijective g :=
-  And.imp LeftInverse.injective RightInverse.surjective
+@[grind =>] theorem leftInverse_of_leftInverse_of_injective (h : f.LeftInverse g)
+    (hf : Injective f) : LeftInverse g f := by
+  simp only [LeftInverse, hf.eq_iff.symm, h.apply_apply, implies_true]
 
-theorem IsEquiv.bijective_left : IsEquiv f g → Bijective f :=
-  IsEquiv.bijective_right ∘ And.symm
+alias LeftInverse.leftInverse_of_injective := leftInverse_of_leftInverse_of_injective
+alias Injective.leftInverse_of_leftInverse := leftInverse_of_leftInverse_of_injective
+
+@[grind =>] theorem leftInverse_of_leftInverse_of_surjective (h : f.LeftInverse g)
+    (hg : Surjective g) : LeftInverse g f := by
+  simp only [LeftInverse, hg.forall, h.apply_apply, implies_true]
+
+alias LeftInverse.leftInverse_of_surjective := leftInverse_of_leftInverse_of_surjective
+alias Surjective.leftInverse_of_leftInverse := leftInverse_of_leftInverse_of_surjective
+
+theorem eq_of_leftInverse_of_leftInverse_of_injective_left (hfg : f.LeftInverse g)
+    (hfg' : f.LeftInverse g') (hf : f.Injective) : g = g' := by grind
+
+theorem eq_of_leftInverse_of_leftInverse_of_surjective_right (hfg : g.LeftInverse f)
+    (hfg' : g'.LeftInverse f) (hf : f.Surjective) : g = g' := by grind
+
+alias Injective.eq_of_leftInverse_of_leftInverse :=
+  eq_of_leftInverse_of_leftInverse_of_injective_left
+alias LeftInverse.eq_of_leftInverse_of_injective :=
+  eq_of_leftInverse_of_leftInverse_of_injective_left
+
+alias Surjective.eq_of_leftInverse_of_leftInverse :=
+  eq_of_leftInverse_of_leftInverse_of_surjective_right
+alias LeftInverse.eq_of_leftInverse_of_surjective :=
+  eq_of_leftInverse_of_leftInverse_of_surjective_right
+
+theorem isBijective_of_leftInverse_of_bijective_right (hfg : f.LeftInverse g) (hg : g.Bijective) :
+    f.Bijective := by grind
+
+alias LeftInverse.bijective_left_of_bijective_right := isBijective_of_leftInverse_of_bijective_right
+alias Bijective.bijective_left_of_leftInverse := isBijective_of_leftInverse_of_bijective_right
+
+theorem isBijective_of_leftInverse_of_bijective_left (hfg : f.LeftInverse g) (hg : f.Bijective) :
+    g.Bijective := by grind
+
+alias LeftInverse.bijective_right_of_bijective_left := isBijective_of_leftInverse_of_bijective_left
+alias Bijective.bijective_right_of_leftInverse := isBijective_of_leftInverse_of_bijective_left
+
+end LeftInverse
+
+section Inverse
+
+variable {f : α → β} {g : β → α}
+
+attribute [grind =>] Inverse.leftInverse Inverse.rightInverse
+
+theorem Inverse.bijective_right (h : Inverse f g) : Bijective g := by grind
+
+theorem Inverse.bijective_left (h : Inverse f g) : Bijective f := by grind
+
+@[grind =>]
+theorem inverse_of_leftInverse_of_leftInverse (hfg : f.LeftInverse g)
+    (hgf : g.LeftInverse f) : f.Inverse g := ⟨hfg, hgf⟩
+
+alias LeftInverse.inverse_of_leftInverse := inverse_of_leftInverse_of_leftInverse
+
+theorem inverse_iff_leftInverse_rightInverse : f.Inverse g ↔ f.LeftInverse g ∧ g.LeftInverse f := by
+  grind
+
+theorem Inverse.symm : Inverse f g → Inverse g f := by grind
+theorem inverse_comm : Inverse f g ↔ Inverse g f := by grind
+
+theorem inverse_of_leftInverse_of_surjective : f.LeftInverse g → Surjective g ->
+    Inverse f g := by grind
+
+theorem inverse_of_leftInverse_of_injective : f.LeftInverse g → Injective f ->
+    Inverse f g := by grind
+
+alias LeftInverse.inverse_of_surjective := inverse_of_leftInverse_of_surjective
+alias Surjective.inverse_of_leftInverse := inverse_of_leftInverse_of_surjective
+alias LeftInverse.inverse_of_injective := inverse_of_leftInverse_of_injective
+alias Injective.inverse_of_leftInverse := inverse_of_leftInverse_of_injective
+
+theorem Inverse.eq_of_rightInverse (h : f.Inverse g) (h' : f.LeftInverse g') :
+    g = g' := by grind
+
+alias LeftInverse.eq_of_inverse_right := Inverse.eq_of_rightInverse
+
+theorem Inverse.eq_of_leftInverse (h : f.Inverse g) (h' : g'.LeftInverse f) :
+    g = g' := by grind
+
+alias LeftInverse.eq_of_inverse_left := Inverse.eq_of_leftInverse
+
+@[grind =>] theorem Inverse.comp_eq_id_left (h : f.Inverse g) : f ∘ g = id :=
+  h.leftInverse.comp_eq_id
+@[grind =>] theorem Inverse.comp_eq_id_right (h : f.Inverse g) : g ∘ f = id :=
+  h.rightInverse.comp_eq_id
+
+theorem inverse_iff_comps_eq_id : f.Inverse g ↔ f ∘ g = id  ∧ g ∘ f = id := by
+  rw [inverse_iff_leftInverse_rightInverse, leftInverse_iff_comp_eq_id, leftInverse_iff_comp_eq_id]
+
+end Inverse
+
+section HasRightInverse
+
+variable {f : α → β} {g : β → α}
+
+theorem hasRightInverse_iff_exists_leftInverse : HasRightInverse f ↔ ∃ g : β → α, f.LeftInverse g :=
+  Iff.rfl
+
+theorem LeftInverse.hasRightInverse (h : f.LeftInverse g) : HasRightInverse f := ⟨_, h⟩
+
+theorem HasRightInverse.exists_leftInverse : HasRightInverse f → ∃ g : β → α, f.LeftInverse g := id
+
+noncomputable def HasRightInverse.inv (h : HasRightInverse f) : β → α := h.exists_leftInverse.choose
+
+theorem HasRightInverse.leftInverse_inv (h : HasRightInverse f) : f.LeftInverse h.inv :=
+  h.exists_leftInverse.choose_spec
+
+theorem inverse_inv_of_hasRightInverse_of_injective (h : HasRightInverse f) (hs : f.Injective) :
+    f.Inverse h.inv := h.leftInverse_inv.inverse_of_injective hs
+
+alias HasRightInverse.inverse_inv_of_injective := inverse_inv_of_hasRightInverse_of_injective
+alias Injective.inverse_inv_of_hasRightInverse := inverse_inv_of_hasRightInverse_of_injective
+
+theorem Surjective.hasRightInverse (hf : f.Surjective) : f.HasRightInverse :=
+  ⟨_, fun b => (hf b).choose_spec⟩
+
+theorem surjective_iff_hasRightInverse : f.Surjective ↔ f.HasRightInverse :=
+  ⟨Surjective.hasRightInverse, HasRightInverse.surjective⟩
+
+@[simp, grind =>] theorem HasRightInverse.comp_inv (h : HasRightInverse f) : f ∘ h.inv = id :=
+  h.leftInverse_inv.comp_eq_id
+
+end HasRightInverse
+
+section HasLeftInverse
+
+variable {f : α → β} {g : β → α}
+
+theorem hasLeftInverse_iff_exists_leftInverse : HasLeftInverse f ↔ ∃ g : β → α, g.LeftInverse f :=
+  Iff.rfl
+
+theorem LeftInverse.hasLeftInverse (h : f.LeftInverse g) : HasLeftInverse g := ⟨_, h⟩
+
+theorem HasLeftInverse.exists_leftInverse : HasLeftInverse f → ∃ g : β → α, g.LeftInverse f := id
+
+noncomputable def HasLeftInverse.inv (h : HasLeftInverse f) : β → α := h.exists_leftInverse.choose
+
+theorem HasLeftInverse.inv_leftInverse (h : HasLeftInverse f) : h.inv.LeftInverse f :=
+  h.exists_leftInverse.choose_spec
+
+theorem inverse_inv_of_hasLeftInverse_of_surjective (h : HasLeftInverse f) (hs : f.Surjective) :
+    f.Inverse h.inv := (h.inv_leftInverse.inverse_of_surjective hs).symm
+
+alias HasLeftInverse.inverse_inv_of_surjective := inverse_inv_of_hasLeftInverse_of_surjective
+alias Surjective.inverse_inv_of_hasLeftInverse := inverse_inv_of_hasLeftInverse_of_surjective
+
+open Classical in theorem injective_iff_hasLeftInverse [Nonempty (β → α)] :
+    f.Injective ↔ f.HasLeftInverse :=
+  ⟨fun hf => ⟨fun b => if h : ∃ a, f a = b then h.choose else (ofNonempty : β → α) b,
+      (fun a => (dite_eq_left ⟨a, rfl⟩).trans (hf (Exists.choose_spec (p := (f · = f a)) _)))⟩,
+  fun ⟨_, h⟩ => h.injective⟩
+
+@[simp, grind =>] theorem HasLeftInverse.inv_comp (h : HasLeftInverse f) : h.inv ∘ f  = id :=
+  h.inv_leftInverse.comp_eq_id
+
+end HasLeftInverse
+
+section HasInverse
+
+variable {f : α → β} {g : β → α}
+
+theorem hasInverse_iff_exists_inverse : HasInverse f ↔ ∃ g : β → α, g.Inverse f := Iff.rfl
+
+theorem Inverse.hasInverse_left (h : f.Inverse g) : f.HasInverse := ⟨_, h.symm⟩
+theorem Inverse.hasInverse_right (h : f.Inverse g) : g.HasInverse := ⟨_, h⟩
+
+theorem HasInverse.exists_leftinverse : HasInverse f → ∃ g : β → α, g.Inverse f := id
+theorem HasInverse.exists_rightInverse : HasInverse f → ∃ g : β → α, f.Inverse g :=
+  Exists.imp (fun _ => Inverse.symm)
+
+noncomputable def HasInverse.inv (h : HasInverse f) : β → α := h.choose
+
+@[grind =>]
+theorem HasInverse.inv_inverse (h : HasInverse f) : h.inv.Inverse f := h.choose_spec
+
+@[grind =>]
+theorem HasInverse.inverse_inv (h : HasInverse f) : f.Inverse h.inv := h.choose_spec.symm
+theorem HasInverse.hasInverse_inv (h : HasInverse f) : HasInverse h.inv := ⟨_, h.inverse_inv⟩
+
+@[grind =>]
+theorem HasInverse.hasLeftInverse (h : HasInverse f) : HasLeftInverse f :=
+  h.imp (fun _ => Inverse.leftInverse)
+
+@[grind =>]
+theorem HasInverse.hasRightInverse (h : HasInverse f) : HasRightInverse f :=
+  h.imp (fun _ => Inverse.rightInverse)
+
+@[grind =>]
+theorem inverse_of_hasLeftInverse_of_hasRightInverse (hl : HasLeftInverse f)
+    (hr : HasRightInverse f) : HasInverse f :=
+  hl.imp fun _ h => h.inverse_of_surjective hr.surjective
+
+alias HasLeftInverse.hasInverse_of_hasRightInverse := inverse_of_hasLeftInverse_of_hasRightInverse
+alias HasRightInverse.hasInverse_of_hasLeftInverse := inverse_of_hasLeftInverse_of_hasRightInverse
+
+@[grind =>]
+theorem HasInverse.bijective (h : HasInverse f) : f.Bijective :=
+  h.inverse_inv.bijective_left
+
+@[grind =>]
+theorem Bijective.hasInverse (hf : f.Bijective) : f.HasInverse :=
+    (hf.surjective.hasRightInverse.leftInverse_inv.inverse_of_injective
+    hf.injective).hasInverse_left
+
+@[simp, grind =>] theorem HasInverse.comp_inv (h : HasInverse f) : f ∘ h.inv = id :=
+  h.inverse_inv.comp_eq_id_left
+
+@[simp, grind =>] theorem HasInverse.inv_comp (h : HasInverse f) : h.inv ∘ f  = id :=
+  h.inverse_inv.comp_eq_id_right
+
+@[simp] theorem HasInverse.hasRightInverse_inv (h : HasInverse f) : h.hasRightInverse.inv = h.inv :=
+  h.bijective.eq_of_comp_left_eq (by simp)
+
+@[simp] theorem HasInverse.hasLeftInverse_inv (h : HasInverse f) : h.hasLeftInverse.inv = h.inv :=
+  h.bijective.eq_of_comp_right_eq (by simp)
+
+theorem bijective_iff_hasInverse : f.Bijective ↔ f.HasInverse :=
+  ⟨Bijective.hasInverse, HasInverse.bijective⟩
+
+theorem hasInverse_iff_hasRightInverse_hasLeftInverse :
+    HasInverse f ↔ HasLeftInverse f ∧ HasRightInverse f :=
+  ⟨fun h => And.intro h.hasLeftInverse h.hasRightInverse,
+  fun ⟨hi, hs⟩ => hi.hasInverse_of_hasRightInverse hs⟩
+
+end HasInverse
+
+section Idempotent
+
+variable {f : α → α}
+
+theorem Idempotent.apply_apply (hf : f.Idempotent) (i) : f (f i) = f i := hf i
+theorem Idempotent.apply_of_exists_apply (hf : f.Idempotent) {i : α} (hi : ∃ a, f a = i) :
+    f i = i := hi.choose_spec ▸ hf.apply_apply _
+
+@[simp, grind =>]
+theorem Idempotent.restrict_leftInverse_val (hf : f.Idempotent) :
+    f.restrict.LeftInverse Subtype.val := fun ⟨_, hi⟩ => Subtype.ext (hf.apply_of_exists_apply hi)
+
+theorem idempotent_iff : f.Idempotent ↔
+    ∃ (β : Sort (max 1 u)) (p : α → β) (q : β → α), p.LeftInverse q ∧ q ∘ p = f := by grind
+
+end Idempotent
