FinitePerm/Function/Fin.lean
@@ -13,10 +13,13 @@ public import FinitePerm.Function.Swap
 namespace Function
 
 open Fin in
+@[grind =>]
 theorem Injective.bijective_of_ge_fin {f : Fin n → Fin m} (hf : f.Injective) (h : m ≤ n) :
     f.Bijective ∧ n = m := by
   induction m generalizing n with
-  | zero => exact ⟨⟨hf, (·.elim0)⟩, Nat.eq_zero_of_not_pos fun hf => (f ⟨0, hf⟩).elim0⟩
+  | zero =>
+    exact ⟨hf.bijective_of_surjective
+      (·.elim0), Nat.eq_zero_of_not_pos fun hf => (f ⟨0, hf⟩).elim0⟩
   | succ m IH =>
     rcases Nat.exists_eq_add_of_lt h with ⟨k, rfl⟩
     let g := swapVal (last m) (f (last (m + k)))
@@ -29,42 +32,44 @@ theorem Injective.bijective_of_ge_fin {f : Fin n → Fin m} (hf : f.Injective) (
       · intro i
         rcases hFbij.surjective i with ⟨t, rfl⟩
         exact ⟨t.castSucc, Fin.ext rfl⟩
-    exact ⟨⟨hf, fun a => (hgf (g a)).imp fun _ hx => swapVal_bijective.injective hx⟩, by omega⟩
+    exact ⟨hf.bijective_of_surjective
+      (fun a => (hgf (g a)).imp fun _ hx => swapVal_bijective.injective hx), by omega⟩
 
 theorem Injective.bijective_fin {f : Fin n → Fin n} (hf : f.Injective) : f.Bijective :=
   (hf.bijective_of_ge_fin (Nat.le_refl _)).1
 
+@[grind =>]
 theorem Surjective.bijective_of_le_fin {f : Fin n → Fin m} (hf : f.Surjective)
     (h : n ≤ m) : f.Bijective ∧ n = m := by
   let g (y : Fin m) : Fin n := (hf y).choose
-  have hg : f.IsSplitting g := fun y => (hf y).choose_spec
-  obtain ⟨hgBij, hmn⟩ := hg.injective.bijective_of_ge_fin h
-  exact ⟨⟨(hg.isSplitting_of_surjective hgBij.surjective).injective, hf⟩, hmn.symm⟩
+  have hg : f.LeftInverse g := fun y => (hf y).choose_spec
+  grind
 
-theorem Surjective.bijective_fin {f : Fin n → Fin n} (hf : f.Surjective) : f.Bijective :=
-  (hf.bijective_of_le_fin (Nat.le_refl _)).1
+theorem Surjective.bijective_fin {f : Fin n → Fin n} (hf : f.Surjective) : f.Bijective := by
+  grind
 
-@[simp] theorem injective_iff_bijective_fin {f : Fin n → Fin n} : f.Injective ↔ f.Bijective :=
-  ⟨Injective.bijective_fin, Bijective.injective⟩
+@[simp] theorem injective_iff_bijective_fin {f : Fin n → Fin n} : f.Injective ↔ f.Bijective := by
+  grind
 
-@[simp] theorem surjective_iff_bijective_fin {f : Fin n → Fin n} : f.Surjective ↔ f.Bijective :=
-  ⟨Surjective.bijective_fin, Bijective.surjective⟩
+@[simp] theorem surjective_iff_bijective_fin {f : Fin n → Fin n} :
+    f.Surjective ↔ f.Bijective := by grind
 
-theorem IsSplitting.isSplitting_fin {f g : Fin n → Fin n} (h : f.IsSplitting g) :
-    g.IsSplitting f := h.isSplitting_of_surjective h.injective.bijective_fin.surjective
+theorem LeftInverse.leftInverse_fin {f g : Fin n → Fin n} (h : f.LeftInverse g) :
+    g.LeftInverse f := by grind
 
-theorem IsSplitting.isEquiv_fin {f g : Fin n → Fin n} (hf : f.IsSplitting g) : f.IsEquiv g :=
-  hf.isEquiv_of_injective hf.surjective.bijective_fin.injective
+theorem LeftInverse.inverse_fin {f g : Fin n → Fin n} (hf : f.LeftInverse g) : f.Inverse g := by
+  grind
 
-@[simp] theorem isSplitting_iff_isEquiv_fin {f g : Fin n → Fin n} :
-    f.IsSplitting g ↔ f.IsEquiv g := (and_iff_left_of_imp IsSplitting.isSplitting_fin).symm
+@[simp] theorem leftInverse_iff_inverse_fin {f g : Fin n → Fin n} :
+    f.LeftInverse g ↔ f.Inverse g := by grind
 
 def finInv (f : Fin n → Fin n) : Fin n → Fin n := fun i => (Fin.find? (f · == i)).getD i
 
-theorem Bijective.isEquiv_finInv {f : Fin n → Fin n} (hf : f.Bijective) :
-    f.IsEquiv (finInv f) := IsSplitting.isEquiv_fin <| fun i => by
+@[grind .]
+theorem Surjective.inverse_finInv {f : Fin n → Fin n} (hf : f.Surjective) :
+    f.Inverse (finInv f) := LeftInverse.inverse_fin <| fun i => by
   have h : (Fin.find? (f · == i)).isSome :=
-    Fin.isSome_find?_of_eq_true (beq_of_eq (hf.surjective i).choose_spec)
+    Fin.isSome_find?_of_eq_true (beq_of_eq (hf i).choose_spec)
   exact eq_of_beq <| (congrArg (f · == i) (Option.get_eq_getD _).symm).trans
     (Fin.get_find?_eq_true h)
 
